vType: progress towards mkCohPainting

theories/νType/νType.v
@@ -618,12 +618,40 @@ Definition mkCohFrames {E'}:
 Proof.
 Admitted.
 
-Definition mkCohPainting' {E'} {p} {Hp: p.+1 <~ n.+1} r q {Hpq: p.+1 <~ q.+1}
-  {Hpr: p.+2 <~ r.+2} {Hrq: r <~ q} {Hr: r.+2 <~ n.+2} {Hq: q.+1 <~ n.+1}
-  {ε ω} :=
-  (C.(data) D.1).(cohPainting) r q (p := p) (Hp := Hp) (Hpq := Hpq)
-  (Hpr := Hpr) (Hrq := Hrq) (Hr := Hr) (Hq := Hq) (ε := ε) (ω := ω)
-  (E' := D.2) (E := E').
+Let mkFrame {E'} p {Hp: p <~ n.+3} :=
+  Frame n.+1 mkFrame'' mkPainting'' mkRestrFrames' E' mkRestrPainting'
+  mkCohFrames p (Hp := Hp).
+
+Let mkRestrFrame {E'} p {Hp: p.+1 <~ n.+3} q {Hpq: p <~ q}
+  {Hq: q <~ n.+2} ε (d: mkFrame p) :=
+  RestrFrame n.+1 mkFrame'' mkPainting'' mkRestrFrames' E' mkRestrPainting'
+  mkCohFrames p q ε d (Hp := Hp) (Hpq := Hpq) (Hq := Hq).
+
+Let mkPainting {E'} p {Hp: p <~ n.+3} {E} (d: mkFrame p) :=
+  Painting n.+1 mkFrame'' mkPainting'' mkRestrFrames' E'
+  mkRestrPainting' mkCohFrames p d (Hp := Hp) (E := E).
+
+Definition mkRestrPainting {E'} p {Hp: p.+1 <~ n.+3} q {Hpq: p <~ q}
+  {Hq: q <~ n.+2} ε {E} {d: mkFrame p}:
+  mkPainting p d -> mkPainting' p (mkRestrFrame p q ε
+    (Hp := Hp) (Hpq := Hpq) (Hq := Hq) d) :=
+  RestrPainting n.+1 mkFrame'' mkPainting'' mkRestrFrames' E' mkRestrPainting'
+    mkCohFrames p q ε (Hp := Hp) (Hpq := Hpq) (Hq := Hq) (E := E) d.
+
+Definition mkCohFrame {p} {Hp: p.+2 <~ n.+2} r q {Hpq: p.+1 <~ q.+1}
+  {Hpr Hrq Hr Hq} {ε ω} d :=
+  (C.(data) D.1).(cohFrame) (E' := D.2) r q d (Hp := Hp) (Hpq := Hpq)
+  (Hpr := Hpr) (Hrq := Hrq) (Hr := Hr) (Hq := Hq) (ε := ε) (ω := ω).
+
+Definition mkCohPainting {p} {Hp: p.+1 <~ n.+2} r q {Hpq: p.+1 <~ q.+1}
+  {Hpr: p.+2 <~ r.+2} {Hrq: r <~ q} {Hr: r.+2 <~ n.+3} {Hq: q.+1 <~ n.+2}
+  {ε ω} {E d} c: rew [mkPainting'' p] mkCohFrame r q d
+  (Hpr := leI_lower_both Hpr)
+  (Hrq := leI_raise_both Hrq) in
+  mkRestrPainting' p q ε (mkRestrPainting p r ω c
+  (Hq := leI_down (leI_lower_both Hr))) =
+  mkRestrPainting' p r ω (mkRestrPainting p q.+1 ε c
+  (Hpq := leI_down Hpq) (Hq := Hq)).
 
 End νTypeData.
 
@@ -638,7 +666,7 @@ Proof.
   now eapply mkRestrFrames'.
   now eapply mkRestrPainting'.
   now eapply mkCohFrames.
-  (* now eapply mkCohPainting'. *)
+  now eapply mkCohPainting.
 Admitted.
 
 Definition mkCohLayer {n} {C: νType n} {p r q} {Hpr: p.+3 <= r.+3}
